{"nbformat":4,"nbformat_minor":0,"metadata":{"colab":{"provenance":[],"authorship_tag":"ABX9TyM5nm/sLbc6vL3tzsfwxvxo"},"kernelspec":{"name":"python3","display_name":"Python 3"},"language_info":{"name":"python"}},"cells":[{"cell_type":"markdown","source":["Let's explore how functions change based on input size. Specifically, if we double the size of the input, what happens to the value of the function?"],"metadata":{"id":"0fqGm-WwiuTt"}},{"cell_type":"markdown","source":["Compare $f(n)$ with $f(2n)$ to observe the effect of doubling the input size.\n","\n","*  **Constant:** $f(n) = 42$. Then $f(2n) = 42$. The value doesn't change at all.\n","*  **Logarithmic:** $f(n) = \\log_2 (n)$. Then $f(2n) = \\log_2 (2n) = \\log_2 2 + \\log_2 n = 1 + \\log_2 n = f(n) + 1$\n","*  **Linear:** $f(n) = n$. Then $f(2n) = 2n = 2f(n)$. The value also doubles.\n","*  **Linearithmic:** $f(n) = n \\log_2 (n)$. Then $f(2n) = 2n \\log_2 (2n) = 2n \\log_2 2 + 2n\\log_2 n = 2f(n) + 2n$. The value will double and also add $2n$ as well.\n","*  **Quadratic:** $f(n) = n^2$. Then $f(2n) = (2n)^2 = 4n^2 = 4f(n)$. The value increases by 4 times.\n","*  **Cubic:** $f(n) = n^3$. Then $f(2n) = (2n)^3 = 8n^3 = 8f(n)$. The value increases by 8 times.\n","*  **Polynomial of degree-$k$:** $f(n) = n^k$. Then $f(2n) = (2n)^k = 2^k n^k = 2^k f(n)$. The values increases by $2^k$ times\n","*  **Exponential:** $f(n) = 2^n$. Then $f(2n) = 2^{2n} = (2^n)^2 = [f(n)]^2$"],"metadata":{"id":"Wf365buUi1Tm"}},{"cell_type":"markdown","source":["Let's try to prove order notation claims using the definition."],"metadata":{"id":"sJGOHotLm9bZ"}},{"cell_type":"markdown","source":["Proving $O()$ bounds (upper bounds)\n","\n","Recall the definition: The statement $f(n) \\in O(g(n))$ means that there exists two constants $n_0 > 0$ and $c > 0$ such that $f(n) \\leq cg(n)$ for all $n \\geq n_0$."],"metadata":{"id":"kkf11MLdnD0O"}},{"cell_type":"markdown","source":["**Example 1:** Show that $n^3 \\in O(n^3)$\n","\n","We know that $n^3 \\leq n^3$ for all $n$.\n","\n","Choosing $c = 1$ and $n_0 = 42$ (anything works), we have $n^3 \\in O(n^3)$."],"metadata":{"id":"OeT-q5oPnOID"}},{"cell_type":"markdown","source":["**Example 2:** Show that $5n^3 \\in O(n^3)$.\n","\n","We have $5n^3 \\leq 5n^3$ for all $n$\n","\n","Choosing $c = 5$ and $n_0 = 42$ (anything works), we have $5n^3 \\in O(n^3)$."],"metadata":{"id":"d_AhlOlsn2pR"}},{"cell_type":"markdown","source":["Some tips:\n","\n","*  Multiplying a positive value by a number $\\geq 1$ will cause the value to be greater than or equal to the original value. Mathematically, for positive $p$ and $q \\geq 1$, we have $pq \\geq p$\n","*  For positive $q$, we have $p + q \\geq p$ or $p - q \\leq p$\n","*  When adding or multiplying positive terms, we can replace individual terms with larger terms to make the overall sum/product larger"],"metadata":{"id":"XvzC2xccppo7"}},{"cell_type":"markdown","source":["**Example 3:** Show that $n^3 \\in O(n^4)$.\n","\n","We have $n^3 \\underbrace{\\leq}_{n \\geq 1} n^3 (n) = n^4$\n","\n","Choosing $c = 1$ and $n_0 = 1$ (or bigger), we have $n^3 \\in O(n^4)$."],"metadata":{"id":"W-rJZUt5o0JE"}},{"cell_type":"markdown","source":["**Example 4:** Show that $n^3 + 3n \\in O(n^3)$\n","\n","We have $n^3 + 3n \\underbrace{\\leq}_{n^2 \\geq 1} n^3 + 3n (n^2) = n^3 + 3n^3 = 4n^3$\n","\n","Choosing $c = 4$ and $n_0 = 1$ (or bigger), we have $n^3 + 3n \\in O(n^3)$"],"metadata":{"id":"Qjn4JNOyqghI"}},{"cell_type":"markdown","source":["**Example 5:** Show that $2n^2 + 5n + 8 \\in O(n^4)$\n","\n","We have $2n^2 + 5n + 8 \\underbrace{\\leq}_{n^2 \\geq 1} 2n^2 (n^2) + 5n + 8 \\underbrace{\\leq}_{n^3 \\geq 1} 2n^2 (n^2) + 5n(n^3) + 8 \\underbrace{\\leq}_{n^4 \\geq 1} 2n^2 (n^2) + 5n(n^3) + 8 (n^4) = 2n^4 + 5n^4 + 8n^4 = 15n^4$\n","\n","Choosing $c = 15$ and $n_0 = 1$, we have $2n^2 + 5n + 8 \\in O(n^4)$\n","\n","More concise proof:\n","\n","We have $2n^2 + 5n + 8 \\underbrace{\\leq}_{n^2 \\geq 1, n^3 \\geq 1, n^4 \\geq 1} 2n^2 (n^2) + 5n(n^3) + 8 (n^4) = 2n^4 + 5n^4 + 8n^4 = 15n^4$\n","\n","Choosing $c = 15$ and $n_0 = 1$, we have $2n^2 + 5n + 8 \\in O(n^4)$"],"metadata":{"id":"fW1QEnxRt8A8"}},{"cell_type":"markdown","source":["**Example 6:** Show that $5n + 3\\sqrt{n} + \\log n \\in O(n)$\n","\n","We have $5n + 3\\sqrt{n} + \\log n \\underbrace{\\leq}_{\\sqrt{n} \\geq 1} 5n + 3\\sqrt{n} (\\sqrt{n}) + \\log n \\leq 5n + 3n + n = 9n$\n","\n","Choosing $c = 9$ and $n_0 = 1$, we have $5n + 3\\sqrt{n} + \\log n \\in O(n)$"],"metadata":{"id":"uxLcdVUwvdB0"}},{"cell_type":"markdown","source":["**Example 7:** Show that $3n^2 - 8n + 2 \\in O(n^2)$\n","\n","We have $3n^2 - 8n + 2 \\underbrace{\\leq}_{n^2 \\geq 1} 3n^2 - 8n + 2(n^2) \\leq 3n^2 + 2(n^2) = 5n^2$\n","\n","Choosing $c = 5$ and $n_0 = 1$, we have $3n^2 - 8n + 2 \\in O(n^2)$."],"metadata":{"id":"54fgSN82x0Jc"}},{"cell_type":"markdown","source":["**Example 8:** Show that $n! \\in O(n^n)$\n","\n","We have $n! = n \\times (n - 1) \\times (n - 2) \\times \\cdots \\times 3 \\times 2 \\times 1 \\leq \\underbrace{n \\times n \\times n \\times \\cdots \\times n \\times n}_{n \\text{ factors}} = n^n$\n","\n","Choosing $c = 1$ and $n_0 = 1$, we have $n! \\in O(n^n)$"],"metadata":{"id":"dvOhuhCtzYYj"}},{"cell_type":"markdown","source":["We can prove $\\Omega ()$ in a similar manner, except the inequality we are seeking is $f(n) \\geq cg(n)$ instead of $f(n) \\leq cg(n)$.\n","\n","So for $O()$, we tried to change each expression to a larger or equal expression. But for $\\Omega ()$, we try to change each expression to a smaller or equal expression."],"metadata":{"id":"OVOV_kNY4tMe"}},{"cell_type":"markdown","source":["$\\Omega ()$ proofs (Lower Bounds)\n","\n","**Example 9:** Show that $n^2 \\in \\Omega (n^2)$\n","\n","We have $n^2 \\geq n^2$ for all $n$.\n","\n","Choosing $c = 1$ and $n_0 = 1$, we have $n^2 \\in \\Omega (n^2)$"],"metadata":{"id":"FXeS5pN347xd"}},{"cell_type":"markdown","source":["**Example 10:** Show that $7n^3 \\in \\Omega (n^3)$\n","\n","We have $7n^3 \\geq 7n^3$ for all $n$.\n","\n","Choosing $c = 7$ and $n_0 = 1$, we have $7n^3 \\in \\Omega (n^3)$"],"metadata":{"id":"SNbeWI175SjV"}},{"cell_type":"markdown","source":["More tips (symmetric to upper bound tips):\n","\n","*  Dividing a positive value by a number $\\geq 1$ will cause the value to be smaller than or equal to the original value. Mathematically, for positive $p$ and $q \\geq 1$, we have $\\frac{p}{q} \\leq p$\n","*  For positive $q$, we have $p + q \\geq p$ or $p - q \\leq p$ [no change]\n","*  When adding or multiplying positive terms, we can replace individual terms with smaller terms to make the overall sum/product smaller"],"metadata":{"id":"ln7rwxac6kMd"}},{"cell_type":"markdown","source":["**Example 11:** Show that $n^3 \\in \\Omega (n^2)$.\n","\n","We have $n^3 \\underbrace{\\geq}_{n \\geq 1} \\frac{n^3}{n} = n^2$\n","\n","Choosing $c = 1$ and $n_0 = 1$, we have $n^3 \\in \\Omega (n^2)$"],"metadata":{"id":"A7SgiBZx5xjd"}},{"cell_type":"markdown","source":["**Example 12:** Show that $n^8 \\in \\Omega (n^3)$\n","\n","We have $n^8 \\underbrace{\\geq}_{n^5 \\geq 1} \\frac{n^8}{n^5} = n^3$\n","\n","Choosing $c = 1$ and $n_0 = 1$, we have $n^8 \\in \\Omega (n^3)$"],"metadata":{"id":"ZYa_0QbH67AI"}},{"cell_type":"markdown","source":["**Example 13:** Show that $5n^3 + 3n^2 + 7n + 15 \\in \\Omega (n^3)$\n","\n","We have $5n^3 + 3n^2 + 7n + 15 \\geq 5n^3$\n","\n","Choosing $c = 5$ and $n_0 = 1$, we have $5n^3 + 3n^2 + 7n + 15 \\in \\Omega (n^3)$"],"metadata":{"id":"VqW3w9lt7bJH"}},{"cell_type":"markdown","source":["**Example 14:** Show that $5n^3 + 3n^2 + 7n + 15 \\in \\Omega (n)$\n","\n","We have $5n^3 + 3n^2 + 7n + 15 \\geq 7n$\n","\n","Choosing $c = 7$ and $n_0 = 1$, we have $5n^3 + 3n^2 + 7n + 15 \\in \\Omega (n)$"],"metadata":{"id":"ZtiarTBs8SkE"}},{"cell_type":"markdown","source":["**Example 15:** Show that $5n^3 + 3n^2 + 15 \\in \\Omega (n)$\n","\n","We have $5n^3 + 3n^2 + 15 \\geq 5n^3 \\underbrace{\\geq}_{n^2 \\geq 1} \\frac{5n^3}{n^2} = 5n$\n","\n","Choosing $c = 5$ and $n_0 = 1$, we have $5n^3 + 3n^2 + 15 \\in \\Omega (n)$"],"metadata":{"id":"G9TK7lWf8kjt"}},{"cell_type":"markdown","source":["Making a negative term bigger will make the entire expression smaller. How do we make a negative term bigger? Think about what we did for $O()$ proofs, e.g., multiplying by a factor $\\geq 1$"],"metadata":{"id":"a6oIIRGk-45j"}},{"cell_type":"markdown","source":["For $O()$ proofs, you can\n","\n","*  remove negative terms\n","*  [usually not useful] divide negative terms by factors $\\geq 1$\n","*  multiply positive terms with factors $\\geq 1$\n","*  replace positive terms in sum/product with larger terms\n","\n","For $\\Omega ()$ proofs, you can\n","\n","*  remove positive terms\n","*  divide positive terms by factors $\\geq 1$\n","*  multiply negative terms with factors $\\geq 1$\n","*  replace positive terms in sum/product with smaller terms"],"metadata":{"id":"M2QGYYgS_Wlv"}},{"cell_type":"markdown","source":["**Example 16:** Show that $7n^3 - 3n^2 \\in \\Omega (n^3)$\n","\n","We have $7n^3 - 3n^2 \\underbrace{\\geq}_{n \\geq 1} 7n^3 - 3n^2 (n) = 7n^3 - 3n^3 = 4n^3$\n","\n","Choosing $c = 4$ and $n_0 = 1$, we have $7n^3 - 3n^2 \\in \\Omega (n^3)$"],"metadata":{"id":"zjiizqfk98GQ"}},{"cell_type":"markdown","source":["**Example 17:** Show that $7n^3 - 13n^2 \\in \\Omega (n^3)$\n","\n","We have $7n^3 - 13n^2 \\underbrace{\\geq}_{\\frac{n}{13} \\geq 1} 7n^3 - 13n^2 \\left(\\frac{n}{13}\\right) = 7n^3 - n^3 = 6n^3$\n","\n","This proof requires $\\frac{n}{13} \\geq 1$, which is equivalent to $n \\geq 13$\n","\n","Choosing $c = 6$ and $n_0 = 13$ (or bigger), we have $7n^3 - 13n^2 \\in \\Omega (n^3)$"],"metadata":{"id":"o4CCYpYZAfpE"}},{"cell_type":"markdown","source":["**Example 18:** Show that $n^3 - 60n \\in \\Omega (n^3)$\n","\n","We have $n^3 - 60n \\underbrace{\\geq}_{\\frac{n^2}{120} \\geq 1} n^3 - 60n\\left(\\frac{n^2}{120}\\right) = n^3 - \\frac{n^3}{2} = \\frac{n^3}{2}$\n","\n","This proof requires $\\frac{n^2}{120} \\geq 1$, which is equivalent to $n^2 \\geq 120$.\n","\n","Choosing $c = \\frac{1}{2}$ and $n_0 = 11$ (anything above $\\sqrt{120}$), we have $n^3 - 60n \\in \\Omega (n^3)$"],"metadata":{"id":"qyouufW9DW5i"}},{"cell_type":"markdown","source":["**Example 19:** Show that $\\frac{3n^5 + 9n^3 - 4}{n^2 - 5n + 8} \\in O(n^3)$\n","\n","We have $\\frac{3n^5 + 9n^3 - 4}{n^2 - 5n + 8} \\underbrace{\\leq}_{n^2 \\geq 1} \\frac{3n^5 + 9n^3(n^2)}{n^2 - 5n + 8} \\underbrace{\\leq}_{n/10 \\geq 1} \\frac{3n^5 + 9n^3(n^2)}{n^2 - 5n(n/10)} = \\frac{12n^5}{n^2/2} = 24n^3$\n","\n","This proof requires both $n^2 \\geq 1$ and $n/10 \\geq 1$. Choosing $n \\geq 10$ satisfies both conditions.\n","\n","Choosing $c = 24$ and $n_0 = 10$, we have $\\frac{3n^5 + 9n^3 - 4}{n^2 - 5n + 8} \\in O(n^3)$"],"metadata":{"id":"VYE36PL_GJT6"}},{"cell_type":"markdown","source":["**Example 20:** Show that $\\frac{3n^5 + 9n^3 - 4}{n^2 - 5n + 8} \\in \\Omega(n^3)$\n","\n","We have $\\frac{3n^5 + 9n^3 - 4}{n^2 - 5n + 8} \\underbrace{\\geq}_{(n^5/4) \\geq 1} \\frac{3n^5 - 4(n^5/4)}{n^2 - 5n + 8} \\underbrace{\\geq}_{n^2 \\geq 1} \\frac{3n^5 - 4(n^5/4)}{n^2+ 8(n^2)} = \\frac{2n^5}{9n^2} = \\frac{2n^3}{9}$\n","\n","This proof requires $(n^5/4) \\geq 1$ and $n^2 \\geq 1$. Choosing $n_0 = 10$ satisfies both.\n","\n","Choosing $c = 2/9$ and $n_0 = 10$ (anything above $4^{1/5}$), we have $\\frac{3n^5 + 9n^3 - 4}{n^2 - 5n + 8} \\in \\Omega(n^3)$"],"metadata":{"id":"8zB5uzyVI9yc"}},{"cell_type":"markdown","source":["How do we prove $\\Theta ()$, which is the tight bound?\n","\n","Proving both $O()$ and $\\Omega ()$ is equivalent to proving $\\Theta ()$."],"metadata":{"id":"_uZ0bLhYKtX3"}},{"cell_type":"markdown","source":["**Example 21:** Show that $\\frac{3n^5 + 9n^3 - 4}{n^2 - 5n + 8} \\in \\Theta(n^3)$\n","\n","We showed $\\frac{3n^5 + 9n^3 - 4}{n^2 - 5n + 8} \\in O(n^3)$ in Example 19 and we showed $\\frac{3n^5 + 9n^3 - 4}{n^2 - 5n + 8} \\in \\Omega(n^3)$ in Example 20. Therefore, $\\frac{3n^5 + 9n^3 - 4}{n^2 - 5n + 8} \\in \\Theta(n^3)$"],"metadata":{"id":"jek_41faLEbB"}}]}